refactoring

Dex001/Dex001.fst
@@ -17,7 +17,7 @@ type order = {
     underlyingAmount: U64.t; // amount of collateral for the order
     pairAsset: asset;
     orderTotal: U64.t; // the amount of the pair required to take the entire order
-    makerPubKeyHash: hash // the public key of the order maker
+    makerPubKey: publicKey // the public key of the order maker
 }
 
 // A double uint64, needed for multiplying two arbitrary uint64s without overflow
@@ -60,120 +60,82 @@ let hashPubkey pk = // 4
     Hash.updateByteArray pk Hash.empty // 384
     >>= Hash.finalize // 20
 
-val hashOrder: order -> hash `cost` 1973
-let hashOrder order = // 33
+val hashOrder: order -> hash `cost` 2384
+let hashOrder order = // 36
     let! underlyingAssetHash = hashAsset order.underlyingAsset in // 408
     let! underlyingAmountHash = hashU64 order.underlyingAmount in // 72
     let! pairAssetHash = hashAsset order.pairAsset in // 408
     let! orderTotalHash = hashU64 order.orderTotal in // 72
+    let! makerPubKeyHash = hashPubkey order.makerPubKey in // 408
         Hash.updateHash underlyingAssetHash Hash.empty // 192
     >>= Hash.updateHash underlyingAmountHash // 192
     >>= Hash.updateHash pairAssetHash // 192
     >>= Hash.updateHash orderTotalHash // 192
-    >>= Hash.updateHash order.makerPubKeyHash // 192
+    >>= Hash.updateHash makerPubKeyHash // 192
     >>= Hash.finalize // 20
 
-val getUnderlyingAsset: option (Dict.t data) -> result asset `cost` 241
-let getUnderlyingAsset dict = // 43
-    let! version = dict >!= Dict.tryFind "UnderlyingAssetVersion" // 64
-                        >?= tryU32 in // 2
-    let! contractHash = dict >!= Dict.tryFind "UnderlyingContractHash" // 64
-                             >?= tryHash in // 2
-    let! subID = dict >!= Dict.tryFind "UnderlyingSubIdentifier" // 64
-                      >?= tryHash in // 2
-    match version, contractHash, subID with
-    | Some version, Some contractHash, Some subID ->
-        RT.ok (version, contractHash, subID)
-    | None, _, _ ->
-        RT.failw "Message Body must include valid UnderlyingAssetVersion"
-    | _, None, _ ->
-        RT.failw "Message Body must include valid UnderlyingContractHash"
-    | _, _, None ->
-        RT.failw "Message Body must include valid UnderlyingSubIdentifier"
+val getAsset: option (Dict.t data) -> string -> option asset `cost` 137
+let getAsset dict fieldName = // 7
+    dict >!= Dict.tryFind fieldName // 64
+         >?= tryString // 2
+         >?= Zen.Asset.parse // 64
 
-val getUnderlyingAmount: option (Dict.t data) -> result U64.t `cost` 82
-let getUnderlyingAmount dict = // 16
-    let! underlyingAmount = dict >!= Dict.tryFind "UnderlyingAmount" // 64
-                                 >?= tryU64 in // 2
-    match underlyingAmount with
-    | Some underlyingAmount ->
-        if underlyingAmount <> 0UL
-        then RT.ok underlyingAmount
-        else RT.failw "UnderlyingAmount cannot be 0"
-    | None ->
-        RT.failw "Message Body must include valid UnderlyingAmount"
+val getU64: option (Dict.t data) -> string -> option U64.t `cost` 80
+let getU64 dict fieldName = // 14
+    let! x = dict >!= Dict.tryFind fieldName // 64
+                  >?= tryU64 in // 2
+    ret ( if x <> Some 0UL then x else None )
 
-val getPairAsset: option (Dict.t data) -> result asset `cost` 241
-let getPairAsset dict = // 43
-    let! version = dict >!= Dict.tryFind "PairAssetVersion" // 64
-                        >?= tryU32 in // 2
-    let! contractHash = dict >!= Dict.tryFind "PairContractHash" // 64
-                             >?= tryHash in // 2
-    let! subID = dict >!= Dict.tryFind "PairSubIdentifier" // 64
-                      >?= tryHash in // 2
-    match version, contractHash, subID with
-    | Some version, Some contractHash, Some subID ->
-        RT.ok (version, contractHash, subID)
-    | None, _, _ ->
-        RT.failw "Message Body must include valid PairAssetVersion"
-    | _, None, _ ->
-        RT.failw "Message Body must include valid PairContractHash"
-    | _, _, None ->
-        RT.failw "Message Body must include valid PairSubIdentifier"
+val getHash: option (Dict.t data) -> string -> option hash `cost` 71
+let getHash dict fieldName = // 5
+    dict >!= Dict.tryFind fieldName // 64
+         >?= tryHash // 2
 
-val getOrderTotal: option (Dict.t data) -> result U64.t `cost` 82
-let getOrderTotal dict = // 16
-    let! orderTotal = dict >!= Dict.tryFind "OrderTotal" // 64
-                           >?= tryU64 in // 2
-    match orderTotal with
-    | Some orderTotal ->
-        if  orderTotal <> 0UL
-        then RT.ok orderTotal
-        else RT.failw "OrderTotal cannot be 0"
-    | None ->
-        RT.failw "Message Body must include valid OrderTotal"
+val getMakerPubKey: option (Dict.t data) -> option publicKey `cost` 71
+let getMakerPubKey dict = // 5
+    dict >!= Dict.tryFind "MakerPubKey" // 64
+         >?= tryPublicKey // 2
 
-val getMakerPKHash: option (Dict.t data) -> result hash `cost` 77
-let getMakerPKHash dict = // 11
-    let! makerPKHash = dict >!= Dict.tryFind "MakerPKHash" // 64
-                            >?= tryHash in // 2
-    match makerPKHash with
-    | Some makerPKHash ->
-        RT.ok makerPKHash
-    | None ->
-        RT.failw "Message Body must include valid MakerPKHash"
+val getReturnAddress: option (Dict.t data) -> option lock `cost` 71
+let getReturnAddress dict = // 5
+    dict >!= Dict.tryFind "returnAddress" // 64
+                              >?= tryLock // 2
 
-val getReturnAddress: option (Dict.t data) -> result lock `cost` 77
-let getReturnAddress dict = // 11
-    let! returnAddress = dict >!= Dict.tryFind "returnAddress" // 64
-                              >?= tryLock in // 2
-    match returnAddress with
-    | Some returnAddress ->
-        RT.ok returnAddress
-    | None ->
-        RT.failw "Message Body must include valid returnAddress"
+val getOrder: option (Dict.t data) -> result order `cost` 570
+let getOrder dict = // 65
+    let! underlyingAsset = getAsset dict "UnderlyingAsset" in // 137
+    let! underlyingAmount = getU64 dict "UnderlyingAmount" in // 80
+    let! pairAsset = getAsset dict "PairAsset"in // 137
+    let! orderTotal = getU64 dict "OrderTotal" in // 80
+    let! makerPubKey = getMakerPubKey dict in // 71
+    match underlyingAsset, underlyingAmount, pairAsset, orderTotal, makerPubKey with
+    | Some underlyingAsset, Some underlyingAmount,
+      Some pairAsset, Some orderTotal, Some makerPubKey ->
+        RT.ok ({ underlyingAsset=underlyingAsset;
+                 underlyingAmount=underlyingAmount;
+                 pairAsset=pairAsset;
+                 orderTotal=orderTotal;
+                 makerPubKey=makerPubKey })
+    | None, _, _, _, _ -> RT.autoFailw "Could not parse UnderlyingAsset"
+    | _, None, _, _, _ -> RT.autoFailw "Could not parse UnderlyingAmount, or UnderlyingAmount was 0"
+    | _, _, None, _, _ -> RT.autoFailw "Could not parse PairAsset"
+    | _, _, _, None, _ -> RT.autoFailw "Could not parse OrderTotal, or OrderTotal was 0"
+    | _, _, _, _, None -> RT.autoFailw "Could not parse MakerPubKey"
 
-val getOrderAsset: contractId -> order -> asset `cost` 1982
+val getOrderAsset: contractId -> order -> asset `cost` 2393
 let getOrderAsset contractID order = // 5
-    let! orderHash = hashOrder order in // 1973
+    let! orderHash = hashOrder order in // 2384
     mkAsset contractID orderHash // 4
 
-val getRequestedPayout: option (Dict.t data) -> result U64.t `cost` 82
-let getRequestedPayout dict = // 16
-    let! requestedPayout = dict >!= Dict.tryFind "RequestedPayout" // 64
-                                >?= tryU64 in // 2
-    match requestedPayout with
-    | Some requestedPayout ->
-        if requestedPayout <> 0UL
-        then RT.ok requestedPayout
-        else RT.failw "RequestedPayout cannot be 0"
-    | None ->
-        RT.failw "Message Body must include valid RequestedPayout"
+val lockToPubKey: asset -> U64.t -> publicKey -> txSkeleton -> txSkeleton `cost` 479
+let lockToPubKey asset amount pubKey tx = // 7
+    let! pubKeyHash = hashPubkey pubKey in // 408
+    TX.lockToPubKey asset amount pubKeyHash tx // 64
 
 // mints an order asset and locks it to the contract, as well as the underlying
-val createOrder: order -> contractId -> txSkeleton -> txSkeleton `cost` 2193
+val createOrder: order -> contractId -> txSkeleton -> txSkeleton `cost` 2604
 let createOrder order contractID tx = // 19
-    let! orderAsset = getOrderAsset contractID order in // 1982
+    let! orderAsset = getOrderAsset contractID order in // 2393
     TX.mint 1UL orderAsset tx // 64
     >>= TX.lockToContract orderAsset 1UL contractID // 64
     >>= TX.lockToContract order.underlyingAsset order.underlyingAmount contractID // 64
@@ -185,9 +147,9 @@ val destroyOrder:
     -> contractId
     -> w: wallet
     -> txSkeleton
-    -> CR.t `cost` (W.size w * 256 + 2457)
+    -> CR.t `cost` (W.size w * 256 + 2868)
 let destroyOrder order contractID w tx = // 24
-    let! orderAsset = getOrderAsset contractID order in // 1982
+    let! orderAsset = getOrderAsset contractID order in // 2393
     begin
     // destroy the order
     TX.destroy 1UL orderAsset tx // 64
@@ -201,93 +163,50 @@ let destroyOrder order contractID w tx = // 24
 //////////////////
 // Making an order
 //////////////////
-type makeParams = {
-    makeUnderlyingAsset: asset;
-    makePairAsset: asset;
-    makeOrderTotal: U64.t
-}
 
-val mkMakeParams: asset -> asset -> U64.t -> result makeParams `cost` 4
-let mkMakeParams underlyingAsset pairAsset orderTotal = // 4
-    RT.ok ( { makeUnderlyingAsset=underlyingAsset;
-              makePairAsset=pairAsset;
-              makeOrderTotal=orderTotal } )
+val makeTx: txSkeleton -> contractId -> publicKey -> order -> CR.t `cost` 2698
+let makeTx tx contractID senderPubKey order = // 27
+    let! underlyingReceived = TX.getAvailableTokens order.underlyingAsset tx in // 64
+    let! tx = // issue a token with the hash of the order as the subidentifier,
+              // and lock it to the contract, with the underlying
+              createOrder order contractID tx // 2604
+              >>= CR.ofTxSkel in // 3
+    match underlyingReceived = order.underlyingAmount, senderPubKey = order.makerPubKey with
+    | true, true -> ret tx
+    | false, _ -> RT.failw "Incorrect amount of UnderlyingAsset Received"
+    | _, false -> RT.failw "SenderPubKey must match MakerPubKey"
 
-val parseMake: option data -> result makeParams `cost` 583
-let parseMake messageBody = // 11
-    let! dict = messageBody >!= tryDict in // 4
-    let underlyingAsset = getUnderlyingAsset dict in // 241
-    let pairAsset = getPairAsset dict in // 241
-    let orderTotal = getOrderTotal dict in // 82
-    RT.bind3 underlyingAsset pairAsset orderTotal mkMakeParams // 4
-
-val makeOrder: makeParams -> publicKey -> U64.t -> order `cost` 420
-let makeOrder makeParams senderPK underlyingAmount = // 12
-    let! senderPKHash = hashPubkey senderPK in // 408
-    ret ( { underlyingAsset=makeParams.makeUnderlyingAsset;
-            underlyingAmount=underlyingAmount;
-            pairAsset=makeParams.makePairAsset;
-            orderTotal=makeParams.makeOrderTotal;
-            makerPubKeyHash=senderPKHash } )
-
-val makeTx: txSkeleton -> contractId -> publicKey -> makeParams -> CR.t `cost` 2700
-let makeTx tx contractID senderPK makeParams = // 20
-    let! underlyingAmount = TX.getAvailableTokens makeParams.makeUnderlyingAsset tx in // 64
-    if underlyingAmount <> 0UL then begin
-        let! order = makeOrder makeParams senderPK underlyingAmount in // 420
-        // issue a token with the hash of the order as the subidentifier,
-        // and lock it to the contract, with the underlying
-        createOrder order contractID tx // 2193
-        >>= CR.ofTxSkel // 3
-        end
-    else RT.autoFailw "UnderlyingAmount cannot be 0"
-
-val make: txSkeleton -> contractId -> sender -> option data -> CR.t `cost` 3292
-let make tx contractID sender messageBody = // 9
+val make: txSkeleton -> contractId -> sender -> option data -> CR.t `cost` 3285
+let make tx contractID sender messageBody = // 13
     match sender with
-    | PK senderPK ->
-        let makeParams = parseMake messageBody in // 583
-        makeParams `RT.bind` makeTx tx contractID senderPK // 2700
-    | _ ->
-        RT.autoFailw "Sender must authenticate with public key"
+    | PK senderPubKey ->
+        let! dict = messageBody >!= tryDict in // 4
+        getOrder dict // 570
+        `RT.bind`
+        makeTx tx contractID senderPubKey // 2698
+    | _ -> RT.autoFailw "Must authenticate with PubKey"
 
 //////////////////
 // Cancel an order
 //////////////////
 
-val getCancelOrder: publicKey -> option data -> result order `cost` 1122
-let getCancelOrder makerPK messageBody = // 64
-    let! dict = messageBody >!= tryDict in // 4
-    let! underlyingAsset = getUnderlyingAsset dict in // 241
-    let! underlyingAmount = getUnderlyingAmount dict in // 82
-    let! pairAsset = getPairAsset dict in // 241
-    let! orderTotal = getOrderTotal dict in // 82
-    let! makerPKHash = hashPubkey makerPK in // 408
-    match underlyingAsset, underlyingAmount, pairAsset, orderTotal with
-    | OK underlyingAsset, OK underlyingAmount, OK pairAsset, OK orderTotal ->
-        RT.ok ( { underlyingAsset=underlyingAsset;
-                  underlyingAmount=underlyingAmount;
-                  pairAsset=pairAsset;
-                  orderTotal=orderTotal;
-                  makerPubKeyHash=makerPKHash } )
-    | ERR msg, _, _, _
-    | OK _, ERR msg, _, _
-    | OK _, OK _, ERR msg, _
-    | OK _, OK _, OK _, ERR msg -> RT.failw msg
-    | _ -> RT.failw "Something went wrong! Please file a bug report"
-
 val cancelTx:
     txSkeleton
     -> contractId
     -> w: wallet
+    -> publicKey
     -> order
-    -> CR.t `cost` (W.size w * 256 + 2533)
-let cancelTx tx contractID w order = // 12
-    // lock the underlying to the maker's pk
-    TX.lockToPubKey order.underlyingAsset order.underlyingAmount order.makerPubKeyHash tx // 64
-    // destroy the order
-    >>= destroyOrder order contractID w // W.size w * 256 + 2457
-    <: CR.t `cost` (W.size w * 256 + 2521)
+    -> CR.t `cost` (W.size w * 256 + 3368)
+let cancelTx tx contractID w senderPubKey order = // 21
+    let! tx = // W.size w * 256 + 2932
+        // lock the underlying to the maker's pk
+        lockToPubKey order.underlyingAsset order.underlyingAmount order.makerPubKey tx // 479
+        // destroy the order
+        >>= destroyOrder order contractID w // W.size w * 256 + 2868
+        <: CR.t `cost` (W.size w * 256 + 3347) in
+    if senderPubKey = order.makerPubKey
+    then ret tx
+    else RT.failw "SenderPubKey must match MakerPubKey"
 
 val cancel:
     txSkeleton
@@ -295,13 +214,14 @@ val cancel:
     -> sender
     -> option data
     -> w: wallet
-    -> CR.t `cost` (W.size w * 256 + 3665)
-let cancel tx contractID sender messageBody w = // 10
+    -> CR.t `cost` (W.size w * 256 + 3956)
+let cancel tx contractID sender messageBody w = // 14
     match sender with
-    | PK senderPK ->
-        begin let order = getCancelOrder senderPK messageBody in // 1122
-        order `RT.bind` cancelTx tx contractID w // W.size w * 256 + 2533
-        end <: CR.t `cost` (W.size w * 256 + 3655)
+    | PK senderPubKey ->
+        let! dict = messageBody >!= tryDict in //4
+        begin let order = getOrder dict in // 570
+        order `RT.bind` cancelTx tx contractID w senderPubKey // W.size w * 256 + 3368
+        end <: CR.t `cost` (W.size w * 256 + 3938)
     | _ ->
         RT.autoFailw "Sender must authenticate with public key"
 
@@ -351,28 +271,6 @@ let checkRequestedPayout { underlyingAmount=ua; orderTotal=ot} rp pa = // 77
     // both conditions must hold
     ret (ua_pa_lt_rp_ot_ot && rp_ot_ot_lte_ua_pa_ot)
 
-// parse the messageBody to get the order being taken
-val parseTake: option (Dict.t data) -> result order `cost` 800
-let parseTake dict = // 77
-    let! underlyingAsset = getUnderlyingAsset dict in // 241
-    let! underlyingAmount = getUnderlyingAmount dict in // 82
-    let! pairAsset = getPairAsset dict in // 241
-    let! orderTotal = getOrderTotal dict in // 82
-    let! makerPKHash = getMakerPKHash dict in // 77
-    match underlyingAsset, underlyingAmount, pairAsset, orderTotal, makerPKHash with
-    | OK underlyingAsset, OK underlyingAmount, OK pairAsset, OK orderTotal, OK makerPKHash ->
-         RT.ok ({ underlyingAsset=underlyingAsset;
-                  underlyingAmount=underlyingAmount;
-                  pairAsset=pairAsset;
-                  orderTotal=orderTotal;
-                  makerPubKeyHash=makerPKHash })
-    | ERR msg, _, _, _, _
-    | OK _, ERR msg, _, _, _
-    | OK _, OK _, ERR msg, _, _
-    | OK _, OK _, OK _, ERR msg, _
-    | OK _, OK _, OK _, OK _, ERR msg -> RT.failw msg
-    | _ -> RT.failw "Something went wrong! Please file a bug report"
-
 // updates an order in the case of a partial fill
 val updateOrder:
     contractId
@@ -380,15 +278,15 @@ val updateOrder:
     -> U64.t
     -> U64.t
     -> txSkeleton
-    -> txSkeleton `cost` 2210
+    -> txSkeleton `cost` 2621
 let updateOrder contractID order paymentAmount payoutAmount tx = let open U64 in // 17
     if paymentAmount <^ order.orderTotal // partial fill, so need to update the order
     then // create the new order
         let newOrder = { order with
                          underlyingAmount=order.underlyingAmount-%^payoutAmount;
                          orderTotal=order.orderTotal-%^paymentAmount } in
-        createOrder newOrder contractID tx // 2193
-    else incRet 2193 tx
+        createOrder newOrder contractID tx // 2604
+    else incRet 2604 tx
 
 val takeTx:
     txSkeleton
@@ -398,34 +296,34 @@ val takeTx:
     -> U64.t
     -> order
     -> lock
-    -> CR.t `cost` (W.size w * 256 + 4818)
+    -> CR.t `cost` (W.size w * 256 + 6055)
 let takeTx tx contractID w paymentAmount payoutAmount order returnAddress = // 23
     //  lock the payout to the taker
     TX.lockToAddress order.underlyingAsset payoutAmount returnAddress tx // 64
     // lock the paymentAmount to the maker
-    >>= TX.lockToPubKey order.pairAsset paymentAmount order.makerPubKeyHash // 64
+    >>= lockToPubKey order.pairAsset paymentAmount order.makerPubKey // 479
     //  create a new order if partial fill, locking the remainder of the underlying to the contract
-    >>= updateOrder contractID order paymentAmount payoutAmount // 2210
+    >>= updateOrder contractID order paymentAmount payoutAmount // 2621
     // add inputs from wallet, destroying the order
-    >>= destroyOrder order contractID w // W.size w * 256 + 2457
+    >>= destroyOrder order contractID w // W.size w * 256 + 2868
 
 val take':
     txSkeleton
     -> contractId
     -> w: wallet
-    -> order
     -> U64.t
     -> lock
-    -> CR.t `cost` (W.size w * 256 + 5057)
-let take' tx contractID w order requestedPayout returnAddress = // 20
+    -> order
+    -> CR.t `cost` (W.size w * 256 + 6294)
+let take' tx contractID w requestedPayout returnAddress order = // 20
     //begin
     let! paymentAmount = TX.getAvailableTokens order.pairAsset tx in // 64
     begin
     let! paymentAmountOK = checkRequestedPayout order requestedPayout paymentAmount in // 155
     if paymentAmountOK
-    then takeTx tx contractID w paymentAmount requestedPayout order returnAddress // W.size w * 256 + 4818
-    else RT.incFailw (W.size w * 256 + 4818) "Incorrect requestedPayout"
-    end <: CR.t `cost` (W.size w * 256 + 4973)
+    then takeTx tx contractID w paymentAmount requestedPayout order returnAddress // W.size w * 256 + 6055
+    else RT.incFailw (W.size w * 256 + 6055) "Incorrect requestedPayout"
+    end <: CR.t `cost` (W.size w * 256 + 6210)
     //end <: CR.t `cost` (W.size w * 256 + 6201)
 
 val take:
@@ -433,16 +331,22 @@ val take:
     -> contractId
     -> option data
     -> w: wallet
-    -> CR.t `cost` (W.size w * 256 + 6034)
-let take tx contractID messageBody w = // 14
+    -> CR.t `cost` (W.size w * 256 + 7048)
+let take tx contractID messageBody w = // 29
     let! dict = messageBody >!= tryDict in // 4
-    let order = parseTake dict in // 800
     //begin
-    let requestedPayout = getRequestedPayout dict in // 82
+    let! requestedPayout = getU64 dict "RequestedPayout" in // 80
     //begin
-    let returnAddress = getReturnAddress dict in // 77
-    RT.bind3 order requestedPayout returnAddress (take' tx contractID w) // 5057
-    <: CR.t `cost` (W.size w * 256 + 6016)
+    let! returnAddress = getReturnAddress dict in // 71
+    match requestedPayout, returnAddress with
+    | Some requestedPayout, Some returnAddress ->
+        let order = getOrder dict in // 570
+        order `RT.bind` take' tx contractID w requestedPayout returnAddress // 6294
+        <: CR.t `cost` (W.size w * 256 + 6864)
+    | None, _ ->
+        RT.autoFailw "Could not parse requestedPayout, or requestedPayout was 0"
+    | _, None ->
+        RT.autoFailw "Could not parse returnAddress"
 
 //////////
 // exports
@@ -458,30 +362,30 @@ val main:
     -> w: wallet
     -> option data
     -> CR.t `cost` ( 9 + begin match command with
-                         | "Make" -> 3292
-                         | "Cancel" -> W.size w * 256 + 3665
-                         | "Take" -> W.size w * 256 + 6034
+                         | "Make" -> 3285
+                         | "Cancel" -> W.size w * 256 + 3956
+                         | "Take" -> W.size w * 256 + 7048
                          | _ -> 0 end )
 let main tx _ contractID command sender messageBody w _ = // 9
     begin
     match command with
     | "Make" ->
-        make tx contractID sender messageBody // 3292
+        make tx contractID sender messageBody // 3285
         <: CR.t `cost` begin match command with
-                       | "Make" -> 3292
-                       | "Cancel" -> W.size w * 256 + 3665
-                       | "Take" -> W.size w * 256 + 6034
+                       | "Make" -> 3285
+                       | "Cancel" -> W.size w * 256 + 3956
+                       | "Take" -> W.size w * 256 + 7048
                        | _ -> 0 end
     | "Cancel" ->
-        cancel tx contractID sender messageBody w // W.size w * 256 + 3665
+        cancel tx contractID sender messageBody w // W.size w * 256 + 3956
     | "Take" ->
-        take tx contractID messageBody w // W.size w * 256 + 6034
+        take tx contractID messageBody w // W.size w * 256 + 7048
     | _ ->
         RT.failw "Unrecognised command"
     end <: CR.t `cost` begin match command with
-                       | "Make" -> 3292
-                       | "Cancel" -> W.size w * 256 + 3665
-                       | "Take" -> W.size w * 256 + 6034
+                       | "Make" -> 3285
+                       | "Cancel" -> W.size w * 256 + 3956
+                       | "Take" -> W.size w * 256 + 7048
                        | _ -> 0 end
 
 val cf:
@@ -495,7 +399,7 @@ val cf:
     -> nat `cost` 12
 let cf _ _ command _ _ w _ = // 12
     ret ( 9 + begin match command with
-              | "Make" -> 3292
-              | "Cancel" -> W.size w * 256 + 3665
-              | "Take" -> W.size w * 256 + 6034
+              | "Make" -> 3285
+              | "Cancel" -> W.size w * 256 + 3956
+              | "Take" -> W.size w * 256 + 7048
               | _ -> 0 end )
